commit

Src/Prover/Nat.lean
@@ -3,6 +3,8 @@ import Src.Prover.Func
 namespace prover
 noncomputable section
 
+section union
+
 def Union (a : Set) : Set :=
 filter (some' # ax_union a) # λ b => ∃ c, c ∈ a ∧ b ∈ c
 
@@ -41,6 +43,13 @@ mpr eq_iff_mem # λ b => iff_trans mem_Union # iff_intro
 theorem union_self {a} : a ∪ a = a :=
 mpr eq_iff_mem # λ b => iff_trans mem_union or_self
 
+theorem union_comm {a b} : a ∪ b = b ∪ a :=
+mpr eq_iff_mem # λ c => iff_trans mem_union # iff_trans' mem_union or_symm'
+
+end union
+
+section insert
+
 def insert (a b : Set) : Set :=
 b ∪ singleton a
 
@@ -56,6 +65,38 @@ mp (mp eq_iff_mem (eq_symm h₁) c) h₂
 theorem insert_eq_of_mem {a b} (h : a ∈ b) : insert a b = b :=
 mpr eq_iff_mem # λ c => iff_trans mem_insert # iff_intro
 (λ h₁ => or_elim h₁ id # λ h₂ => eq_rec' (λ x => x ∈ b) h₂ h) (λ h₁ => or_inl h₁)
+
+end insert
+
+section intersect
+
+def Intersect (a : Set) : Set :=
+filter (⋃ a) # λ b => ∀ c, c ∈ a → b ∈ c
+
+prefix:110 (priority := high) "⋂ " => Intersect
+
+theorem mem_Intersect {a b} : b ∈ ⋂ a ↔ b ∈ ⋃ a ∧ ∀ c, c ∈ a → b ∈ c :=
+iff_trans mem_filter iff_refl
+
+def intersect (a b : Set) : Set :=
+⋂ upair a b
+
+infixl:65 (priority := high) " ∩ " => intersect
+
+theorem mem_intersect {a b c} : c ∈ a ∩ b ↔ c ∈ a ∧ c ∈ b :=
+iff_trans mem_Intersect # iff_intro
+(λ h => and_elim h # λ h₁ h₂ => and_intro (h₂ a left_mem_upair) (h₂ b right_mem_upair))
+(λ h => and_intro (mpr mem_union # or_of_and h) # λ d h₁ => or_elim (mp mem_upair h₁)
+  (λ h₂ => mem_of_mem_of_eq' h₂ # and_left h)
+  (λ h₂ => mem_of_mem_of_eq' h₂ # and_right h))
+
+theorem intersect_self {a} : a ∩ a = a :=
+mpr eq_iff_mem # λ b => iff_trans mem_intersect and_self
+
+theorem intersect_comm {a b} : a ∩ b = b ∩ a :=
+mpr eq_iff_mem # λ c => iff_trans mem_intersect # iff_trans' mem_intersect and_symm'
+
+end intersect
 
 def succ (n : Set) : Set :=
 insert n n
@@ -76,3 +117,8 @@ or_iff_or_right # iff_symm mem_one
 
 def nat_like (S : Set) : Prop :=
 0 ∈ S ∧ ∀ n, n ∈ S → succ n ∈ S
+
+theorem is_succ_iff {n1 n} : is_succ n1 n ↔ n1 = succ n :=
+iff_intro
+(λ h => mpr eq_iff_mem # λ a => iff_symm # iff_trans mem_succ # iff_symm # h a)
+(λ h => eq_rec' (λ x => is_succ x n) h succ_is_succ)
